Instances/Joinable.v
@@ -1,23 +1,222 @@
 Require Import Classes.Joinable.
+Require Import Classes.Monad.
 Require Import Classes.PreorderedSet.
+Require Import Coq.Arith.PeanoNat.
 Require Import Coq.Logic.FunctionalExtensionality.
-Require Import Instances.Monad.
 Require Import Instances.Preorder.
 Require Import Language.Statements.
+Require Import Types.AbstractBool.
+Require Import Types.Interval.
+Require Import Types.Maybe.
+Require Import Types.Parity.
+Require Import Types.State.
 Require Import Types.Stores.
+
+Definition parity_join (p1 p2 : parity) : parity :=
+  match p1, p2 with
+  | par_even, par_even => par_even
+  | par_odd, par_odd => par_odd
+  | par_bottom, par_bottom => par_bottom
+  | par_even, par_bottom | par_bottom, par_even => par_even
+  | par_odd, par_bottom | par_bottom, par_odd => par_odd
+  | _, _ => par_top
+  end.
+
+Lemma parity_join_comm : ∀ p1 p2,
+  parity_join p1 p2 = parity_join p2 p1.
+Proof.
+  destruct p1, p2; reflexivity.
+Qed.
+
+Lemma parity_join_assoc : ∀ p1 p2 p3,
+  parity_join p1 (parity_join p2 p3) = parity_join (parity_join p1 p2) p3.
+Proof.
+  intros. destruct_all parity; reflexivity.
+Qed.
+
+Lemma parity_join_upper_bound_left :
+  ∀ p1 p2, preorder p1 (parity_join p1 p2).
+Proof.
+  intros. destruct_all parity; constructor.
+Qed.
+
+Lemma parity_join_upper_bound_right :
+  ∀ p1 p2, preorder p2 (parity_join p1 p2).
+Proof.
+  intros. destruct_all parity; constructor.
+Qed.
+
+Lemma parity_join_refl : ∀ p, parity_join p p = p.
+Proof.
+  destruct p; reflexivity.
+Qed.
+
+Instance parity_joinable : Joinable parity :=
+{
+  join_refl := parity_join_refl;
+  join_upper_bound_left := parity_join_upper_bound_left;
+  join_upper_bound_right := parity_join_upper_bound_right;
+  join_assoc := parity_join_assoc;
+}.
+
+Definition abstract_bool_join(b1 b2 : abstr_bool) : abstr_bool :=
+  match b1, b2 with
+  | ab_true, ab_true => ab_true
+  | ab_false, ab_false => ab_false
+  | ab_true, ab_bottom | ab_bottom, ab_true => ab_true
+  | ab_false, ab_bottom | ab_bottom, ab_false => ab_false
+  | ab_bottom, ab_bottom => ab_bottom
+  | ab_true, ab_false | ab_false, ab_true => ab_top
+  | ab_top, _ | _, ab_top => ab_top
+  end.
+
+Lemma abstract_bool_join_assoc : ∀ b1 b2 b3,
+  abstract_bool_join b1 (abstract_bool_join b2 b3) =
+  abstract_bool_join (abstract_bool_join b1 b2) b3.
+Proof.
+  intros. destruct_all abstr_bool; reflexivity.
+Qed.
+
+Lemma abstract_bool_join_refl : ∀ b,
+  abstract_bool_join b b = b.
+Proof.
+  destruct b; reflexivity.
+Qed.
+
+Lemma abstract_bool_join_upper_bound_left : ∀ b1 b2,
+  preorder b1 (abstract_bool_join b1 b2).
+Proof.
+  intros. destruct_all abstr_bool; constructor.
+Qed.
+
+Lemma abstract_bool_join_upper_bound_right : ∀ b1 b2,
+  preorder b2 (abstract_bool_join b1 b2).
+Proof.
+  intros. destruct_all abstr_bool; constructor.
+Qed.
+
+Instance abstr_bool_joinable : Joinable abstr_bool :=
+{
+  join_refl := abstract_bool_join_refl;
+  join_assoc := abstract_bool_join_assoc;
+  join_upper_bound_left := abstract_bool_join_upper_bound_left;
+  join_upper_bound_right := abstract_bool_join_upper_bound_right;
+}.
+
+Definition interval_join (i j : interval) : interval :=
+  (Nat.min (min i) (min j), Nat.max (max i) (max j)).
+
+Lemma interval_join_assoc : ∀ i1 i2 i3,
+  interval_join i1 (interval_join i2 i3) =
+  interval_join (interval_join i1 i2) i3.
+Proof.
+  intros. unfold interval_join. 
+  destruct i1 as [n1 m1] eqn:H1. 
+  destruct i2 as [n2 m2] eqn:H2. 
+  destruct i3 as [n3 m3] eqn:H3. 
+  repeat rewrite interval_min_Nat_min. 
+  repeat rewrite interval_max_Nat_max. 
+  rewrite Nat.min_assoc, Nat.max_assoc. reflexivity.
+Qed.
+
+Lemma interval_join_refl : ∀ i,
+  interval_join i i = i.
+Proof.
+  intros. unfold interval_join. 
+  rewrite PeanoNat.Nat.min_id, PeanoNat.Nat.max_id. 
+  pose proof interval_increasing.
+  unfold min, max. destruct i. simpl.
+Admitted.
+
+Require Import Omega.
+Lemma interval_join_upper_bound_left : 
+  ∀ i1 i2, preorder i1 (interval_join i1 i2).
+Proof.
+  intros. unfold interval_join. simpl. constructor; simpl.
+  - unfold min; simpl. omega with *.
+  - unfold max; simpl. omega with *.
+Qed.
+
+Lemma interval_join_upper_bound_right :
+  ∀ i1 i2, preorder i2 (interval_join i1 i2).
+Proof.
+  intros. unfold interval_join. constructor; simpl.
+  - unfold min; simpl. omega with *.
+  - unfold max; simpl. omega with *.
+Qed.
+
+Instance interval_joinable : Joinable interval :=
+{
+  join_refl := interval_join_refl;
+  join_assoc := interval_join_assoc;
+  join_upper_bound_left := interval_join_upper_bound_left;
+  join_upper_bound_right := interval_join_upper_bound_right;
+}.
+
+Definition avalue_join (a1 a2 : avalue) : avalue :=
+  match a1, a2 with
+  | VParity p1, VParity p2 => VParity (join_op p1 p2)
+  | VParity _, VAbstrBool _ | VAbstrBool _, VParity _ => VTop
+  | VParity _, VInterval _ | VInterval _, VParity _ => VTop
+  | VParity _, VTop | VTop, VParity _ => VTop
+  | VParity x, VBottom | VBottom, VParity x => VParity x
+  | VAbstrBool b1, VAbstrBool b2 => VAbstrBool (join_op b1 b2)
+  | VAbstrBool _, VInterval _ | VInterval _, VAbstrBool _ => VTop
+  | VAbstrBool _, VTop | VTop, VAbstrBool _ => VTop
+  | VAbstrBool b, VBottom | VBottom, VAbstrBool b => VAbstrBool b
+  | VInterval i1, VInterval i2 => VInterval (join_op i1 i2)
+  | VInterval _, VTop | VTop, VInterval _ => VTop
+  | VInterval i, VBottom | VBottom, VInterval i => VInterval i
+  | VTop, VTop => VTop
+  | VTop, VBottom | VBottom, VTop => VTop
+  | VBottom, VBottom => VBottom
+  end.
+
+Lemma avalue_join_refl : ∀ a, avalue_join a a = a.
+Proof.
+  destruct a; simpl; try rewrite join_refl; reflexivity.
+Qed.
+
+Lemma avalue_join_assoc : ∀ a1 a2 a3,
+  avalue_join a1 (avalue_join a2 a3) = avalue_join (avalue_join a1 a2) a3.
+Proof.
+  intros. destruct_all avalue; simpl; try rewrite join_assoc; reflexivity.
+Qed.
+  
+Lemma avalue_join_upper_bound_left : ∀ a1 a2,
+  preorder a1 (avalue_join a1 a2).
+Proof. Admitted.
+
+Lemma avalue_join_upper_bound_right : ∀ a1 a2,
+  preorder a2 (avalue_join a1 a2).
+Proof. Admitted.
+
+Instance avalue_joinable : Joinable avalue :=
+{
+  join_refl := avalue_join_refl;
+  join_assoc := avalue_join_assoc;
+  join_upper_bound_left := avalue_join_upper_bound_left;
+  join_upper_bound_right := avalue_join_upper_bound_right;
+}.
 
 Definition abstract_store_join
   (ast1 ast2 : abstract_store) : abstract_store :=
-  fun x => VTop.
+  fun x => join_op (ast1 x) (ast2 x).
 
-Lemma abstract_store_join_comm : forall ast1 ast2,
-  abstract_store_join ast1 ast2 = abstract_store_join ast2 ast1.
-Proof. simple_solve. Qed.
+Lemma abstract_store_join_refl : ∀ ast,
+  abstract_store_join ast ast = ast.
+Proof.
+  unfold abstract_store_join. intros. ext.
+  rewrite join_refl. reflexivity.
+Qed.
 
 Lemma abstract_store_join_assoc : forall ast1 ast2 ast3,
   abstract_store_join ast1 (abstract_store_join ast2 ast3) =
   abstract_store_join (abstract_store_join ast1 ast2) ast3.
-Proof. simple_solve. Qed.
+Proof. 
+  intros. unfold abstract_store_join. ext. rewrite join_assoc.
+  reflexivity.
+Qed.
 
 Lemma abstract_store_join_upperbound_left :
     forall s s', preorder s (abstract_store_join s s').
@@ -30,7 +229,7 @@ Lemma abstract_store_join_upperbound_right :
 Proof. eauto with soundness. Qed.
 
 Global Instance abstract_store_joinable : Joinable abstract_store := {
-  join_op := abstract_store_join;
+  join_refl := abstract_store_join_refl;
   join_upper_bound_left := abstract_store_join_upperbound_left;
   join_upper_bound_right := abstract_store_join_upperbound_right;
   join_assoc := abstract_store_join_assoc;
@@ -54,9 +253,14 @@ Proof.
   reflexivity.
 Qed.
 
+Lemma unit_join_refl : ∀ u, unit_join u u = u.
+Proof. 
+  destruct u. reflexivity.
+Qed.
+
 Global Instance unit_joinable : Joinable unit :=
 {
-  join_op := unit_join;
+  join_refl := unit_join_refl;
   join_upper_bound_left := unit_join_upperbound_left;
   join_upper_bound_right := unit_join_upperbound_right;
   join_assoc := unit_join_assoc;
@@ -93,8 +297,15 @@ Section state_joinable.
     reflexivity.
   Qed.
 
+  Lemma state_join_refl : ∀ st,
+    state_join st st = st.
+  Proof.
+    intros. unfold state_join. ext. repeat rewrite join_refl.
+    simpl. rewrite <- surjective_pairing. reflexivity.
+  Qed.
+
   Global Instance state_joinable : Joinable (State S A) := {
-    join_op := state_join;
+    join_refl := state_join_refl;
     join_upper_bound_left := state_join_upper_bound_left;
     join_upper_bound_right := state_join_upper_bound_right;
     join_assoc := state_join_assoc;
@@ -104,40 +315,45 @@ End state_joinable.
 Section maybe_joinable.
   Context {A : Type} `{A_joinable : Joinable A}.
 
-  Definition join_maybe (m n : Maybe A) : Maybe A :=
+  Definition maybe_join (m n : Maybe A) : Maybe A :=
     match m, n with
     | Just x, Just y => Just (join_op x y)
     | _, _ => None
     end.
 
-  Definition join_maybe_left : ∀ m n, preorder m (join_maybe m n).
+  Lemma maybe_join_left : ∀ m n, preorder m (maybe_join m n).
   Proof.
     destruct m, n; simpl; auto with soundness. 
   Qed.
 
-  Definition join_maybe_right : ∀ m n, preorder n (join_maybe m n).
+  Lemma maybe_join_right : ∀ m n, preorder n (maybe_join m n).
   Proof. destruct m, n; simpl; auto with soundness. Qed.
 
-  Definition join_maybe_assoc : ∀ x y z, 
-    join_maybe x (join_maybe y z) = join_maybe (join_maybe x y) z.
+  Lemma maybe_join_assoc : ∀ x y z, 
+    maybe_join x (maybe_join y z) = maybe_join (maybe_join x y) z.
   Proof.
     intros. destruct x, y, z; try reflexivity.
     simpl. rewrite join_assoc. reflexivity.
   Qed.
 
+  Lemma maybe_join_refl : ∀ m, maybe_join m m = m.
+  Proof.
+    destruct m; simpl; try rewrite join_refl; reflexivity.
+  Qed.
+
   Global Instance maybe_joinable : Joinable (Maybe A) :=
   {
-    join_op := join_maybe;
-    join_upper_bound_left := join_maybe_left;
-    join_upper_bound_right := join_maybe_right;
-    join_assoc := join_maybe_assoc;
+    join_refl := maybe_join_refl;
+    join_upper_bound_left := maybe_join_left;
+    join_upper_bound_right := maybe_join_right;
+    join_assoc := maybe_join_assoc;
   }.
 End maybe_joinable.
 
 Section abstract_maybe_joinable.
 Context {A : Type} `{A_joinable : Joinable A}.
 
-Definition join_maybe_abstract
+Definition abstract_maybe_join
   (st1 st2 : AbstractMaybe A) : AbstractMaybe A :=
   match st1, st2 with
   | NoneA, NoneA => NoneA
@@ -148,64 +364,75 @@ Definition join_maybe_abstract
       JustOrNoneA (join_op x y)
   | JustOrNoneA x, JustOrNoneA y => JustOrNoneA (join_op x y)
   end.
-Hint Unfold join_maybe_abstract : soundness.
+Hint Unfold abstract_maybe_join : soundness.
 
-Lemma join_maybe_abstract_upperbound_left : forall st st',
-  preorder st (join_maybe_abstract st st').
+Lemma abstract_maybe_join_upperbound_left : forall st st',
+  preorder st (abstract_maybe_join st st').
 Proof. simple_solve. Qed.
 
-Lemma join_maybe_abstract_upperbound_right : forall st st',
-  preorder st' (join_maybe_abstract st st').
+Lemma abstract_maybe_join_upperbound_right : forall st st',
+  preorder st' (abstract_maybe_join st st').
 Proof. simple_solve. Qed.
 
-Lemma join_maybe_abstract_assoc : ∀ x y z : AbstractMaybe A,
-  join_maybe_abstract x (join_maybe_abstract y z) =
-  join_maybe_abstract (join_maybe_abstract x y) z.
+Lemma abstract_maybe_join_assoc : ∀ x y z : AbstractMaybe A,
+  abstract_maybe_join x (abstract_maybe_join y z) =
+  abstract_maybe_join (abstract_maybe_join x y) z.
 Proof.
   intros. destruct x, y, z; simpl; try reflexivity.
   all: repeat rewrite join_assoc; reflexivity.
 Qed.
 
+Lemma abstract_maybe_join_refl : ∀ am, 
+  abstract_maybe_join am am = am.
+Proof.
+  destruct am; simpl; try rewrite join_refl; reflexivity.
+Qed.
+
 Global Instance abstract_maybe_joinable : Joinable (AbstractMaybe A) := 
 {
-  join_op := join_maybe_abstract;
-  join_upper_bound_left := join_maybe_abstract_upperbound_left;
-  join_upper_bound_right := join_maybe_abstract_upperbound_right;
-  join_assoc := join_maybe_abstract_assoc;
+  join_refl := abstract_maybe_join_refl;
+  join_upper_bound_left := abstract_maybe_join_upperbound_left;
+  join_upper_bound_right := abstract_maybe_join_upperbound_right;
+  join_assoc := abstract_maybe_join_assoc;
 }.
-
 End abstract_maybe_joinable.
 
 Section joinable_pairs.
   Context {A B} `{A_joinable : Joinable A, B_joinable : Joinable B}.
 
-  Definition join_pair (p q : (A*B)%type) : (A*B)%type :=
+  Definition pair_join (p q : (A*B)%type) : (A*B)%type :=
     (join_op (fst p) (fst q), join_op (snd p) (snd q)).
 
-  Lemma join_pair_left : ∀ p q, preorder p (join_pair p q).
+  Lemma pair_join_left : ∀ p q, preorder p (pair_join p q).
   Proof.
     destruct p, q. eauto with soundness.
   Qed.
 
-  Lemma join_pair_right : ∀ p q, preorder q (join_pair p q).
+  Lemma pair_join_right : ∀ p q, preorder q (pair_join p q).
   Proof.
     destruct p, q. eauto with soundness.
   Qed.
 
-  Lemma join_pair_assoc : ∀ x y z, 
-    join_pair x (join_pair y z) = join_pair (join_pair x y) z.
+  Lemma pair_join_assoc : ∀ x y z, 
+    pair_join x (pair_join y z) = pair_join (pair_join x y) z.
   Proof.
     intros. destruct x as [x1 x2], y as [y1 y2], z as [z1 z2]. 
-    unfold join_pair; simpl. repeat rewrite join_assoc.
+    unfold pair_join; simpl. repeat rewrite join_assoc.
+    reflexivity.
+  Qed.
+
+  Lemma pair_join_refl : ∀ p, pair_join p p = p.
+  Proof.
+    destruct p. unfold pair_join. simpl. repeat rewrite join_refl.
     reflexivity.
   Qed.
 
   Global Instance joinable_pairs : Joinable (A*B) :=
   {
-    join_op := join_pair;
-    join_upper_bound_left := join_pair_left;
-    join_upper_bound_right := join_pair_right;
-    join_assoc := join_pair_assoc;
+    join_refl := pair_join_refl;
+    join_upper_bound_left := pair_join_left;
+    join_upper_bound_right := pair_join_right;
+    join_assoc := pair_join_assoc;
   }.
 End joinable_pairs.
 
@@ -219,6 +446,7 @@ Section joinable_maybeT.
     Joinable (MaybeT M A) :=
   {
     join_op := join_op;
+    join_refl := join_refl;
     join_upper_bound_left := join_upper_bound_left;
     join_upper_bound_right := join_upper_bound_right;
     join_assoc := join_assoc;
@@ -235,6 +463,7 @@ Section joinable_maybeAT.
     Joinable (MaybeAT M A) :=
   {
     join_op := join_op;
+    join_refl := join_refl;
     join_upper_bound_left := join_upper_bound_left;
     join_upper_bound_right := join_upper_bound_right;
     join_assoc := join_assoc;
@@ -248,35 +477,40 @@ Section joinable_stateT.
   Context {M_joinable : ∀ T {T_preorder : PreorderedSet T},
     Joinable (M T)}.
 
-  Definition join_stateT (st st' : StateT S M A) : StateT S M A :=
+  Definition stateT_join (st st' : StateT S M A) : StateT S M A :=
     λ x, join_op (st x) (st' x).
 
-  Lemma join_stateT_upper_bound_left : ∀ t t' : StateT S M A,
-    preorder t (join_stateT t t').
+  Lemma stateT_join_upper_bound_left : ∀ t t' : StateT S M A,
+    preorder t (stateT_join t t').
   Proof.
-    intros. unfold join_stateT. constructor. intros. 
+    intros. unfold stateT_join. constructor. intros. 
     apply join_upper_bound_left.
   Qed.
 
-  Lemma join_stateT_upper_bound_right : ∀ t t' : StateT S M A, 
-    preorder t' (join_stateT t t').
+  Lemma stateT_join_upper_bound_right : ∀ t t' : StateT S M A, 
+    preorder t' (stateT_join t t').
   Proof.
-    intros. unfold join_stateT. constructor. intros.
+    intros. unfold stateT_join. constructor. intros.
     apply join_upper_bound_right.
   Qed.
 
-  Lemma join_stateT_assoc : ∀ x y z,
-    join_stateT x (join_stateT y z) = join_stateT (join_stateT x y) z.
+  Lemma stateT_join_assoc : ∀ x y z,
+    stateT_join x (stateT_join y z) = stateT_join (stateT_join x y) z.
   Proof.
-    intros. unfold join_stateT. extensionality s.
-    rewrite join_assoc. reflexivity.
+    intros. unfold stateT_join. ext. rewrite join_assoc. reflexivity.
+  Qed.
+
+  Lemma stateT_join_refl : ∀ st,
+    stateT_join st st = st.
+  Proof.
+    intros. unfold stateT_join. ext. rewrite join_refl. reflexivity.
   Qed.
 
   Global Instance stateT_joinable : Joinable (StateT S M A) :=
   {
-    join_op := join_stateT;
-    join_upper_bound_left := join_stateT_upper_bound_left;
-    join_upper_bound_right := join_stateT_upper_bound_right;
-    join_assoc := join_stateT_assoc;
+    join_refl := stateT_join_refl;
+    join_upper_bound_left := stateT_join_upper_bound_left;
+    join_upper_bound_right := stateT_join_upper_bound_right;
+    join_assoc := stateT_join_assoc;
   }.
 End joinable_stateT.
