Types/Interval.v
@@ -1,16 +1,17 @@
 Require Export Base.
-Require Import Types.AbstractBool.
-Require Import Coq.Arith.Plus.
+Require Import Coq.Arith.Le.
 Require Import Coq.Arith.Mult.
 Require Import Coq.Arith.PeanoNat.
+Require Import Coq.Arith.Plus.
+Require Import Omega.
+Require Import Types.AbstractBool.
 
 Definition interval := (nat * nat) % type.
 
-Definition min (i : interval) : nat := 
-  if (Nat.leb (fst i) (snd i)) then (fst i) else (snd i).
-Definition max (i : interval) : nat := 
-  if (Nat.leb (fst i) (snd i)) then (snd i) else (fst i).
-
+Definition min (i : interval) : nat := Nat.min (fst i) (snd i).
+  (*if (Nat.leb (fst i) (snd i)) then (fst i) else (snd i).*)
+Definition max (i : interval) : nat := Nat.max (fst i) (snd i).
+  (*if (Nat.leb (fst i) (snd i)) then (snd i) else (fst i).*)
 
 Definition iplus (i1 i2 : interval) : interval := 
   ((min i1) + (min i2), (max i1) + (max i2)).
@@ -37,36 +38,35 @@ Definition ileqb (i1 i2 : interval) : abstr_bool :=
   else
     ab_top.
 
-
-Require Import Coq.Arith.Le.
 Lemma interval_increasing : forall i,
   min i <= max i.
 Proof with auto with arith.
-  destruct i as [n m]. unfold min, max. simpl.
-  generalize dependent n.
-  induction m...
-  - intro n. induction n...
-  - induction n... simpl. 
-    destruct (Nat.leb n m) eqn:Hnm.
-    apply le_n_S. apply Nat.leb_le. apply Hnm.
-    constructor. apply Nat.leb_gt. apply Hnm.
+  destruct i as [n m]. unfold min, max. simpl. 
+  eapply Nat.le_trans. apply Nat.le_min_l. apply Nat.le_max_l.
 Qed.
 
-Lemma interval_min_l : forall i j : interval,
-  min i <= max i + max j ->
-  min (min i, max i + max j) = min i.
+Lemma interval_min_l : forall i : interval,
+  (*min i <= max i + max j ->*)
+  min (min i, max i) = min i.
 Proof.
-  intros i j H. unfold min, max in *. 
-  destruct (fst i <=? snd i) eqn:Hi; simpl;
-  destruct (fst j <=? snd j) eqn:Hj; simpl.
-  - destruct (fst i <=? snd i + snd j) eqn:Hplus; try reflexivity.
-    apply Nat.leb_nle in Hplus. exfalso. apply Hplus. apply H.
-  - destruct (fst i <=? snd i + fst j) eqn:Hplus; try reflexivity.
-    apply Nat.leb_nle in Hplus. exfalso. apply Hplus. apply H.
-  - destruct (snd i <=? fst i + snd j) eqn:Hplus; try reflexivity.
-    apply Nat.leb_nle in Hplus. exfalso. apply Hplus. apply H.
-  - destruct (snd i <=? fst i + fst j) eqn:Hplus; try reflexivity.
-    apply Nat.leb_nle in Hplus. exfalso. apply Hplus. apply H.
+  intros i. 
+  unfold min, max in *; simpl. 
+  omega with *.
+Qed.
+Hint Rewrite interval_min_l : soundness.
+
+Lemma interval_min_Nat_min : ∀ i j,
+  (min (Nat.min (min i) (min j), Nat.max (max i) (max j))) =
+  Nat.min (min i) (min j).
+Proof.
+  intros. unfold min, max. simpl. omega with *.
+Qed.
+
+Lemma interval_max_Nat_max : ∀ i j,
+  (max (Nat.min (min i) (min j),
+        Nat.max (max i) (max j))) = Nat.max (max i) (max j).
+Proof.
+  intros. unfold min, max. simpl. omega with *.
 Qed.
 
 Lemma interval_min_plus : forall i j,
@@ -75,8 +75,7 @@ Proof.
   destruct i as [li ui], j as [lj uj]. unfold iplus.
   assert (min (li, ui) + min(lj, uj) <= max(li,ui) + max(lj,uj)).
   { apply Coq.Arith.Plus.plus_le_compat; apply interval_increasing. }
-  unfold min at 1. simpl. apply Nat.leb_le in H. rewrite H.
-  reflexivity.
+  unfold min, max in *. simpl. apply Nat.leb_le in H. omega with *.
 Qed.
 
 Lemma interval_max_plus : forall i j,
@@ -85,21 +84,21 @@ Proof.
   unfold iplus. intros i j.
   assert (min i + min j <= max i + max j).
   { apply Coq.Arith.Plus.plus_le_compat; apply interval_increasing. }
-  unfold max at 1. simpl. apply Nat.leb_le in H. rewrite H.
-  reflexivity.
+  unfold max at 1. simpl. apply Nat.leb_le in H. unfold min, max in *.
+  omega with *.
 Qed.
 
 Lemma interval_min_refl : forall i,
   min (i,i) = i.
 Proof.
-  intro. unfold min. simpl. destruct (i <=? i); reflexivity.
+  intro. unfold min. simpl. rewrite Nat.min_id. reflexivity.
 Qed.
 Hint Rewrite interval_min_refl : soundness.
 
 Lemma interval_max_refl : forall i,
   max (i,i) = i.
 Proof.
-  intro. unfold max. simpl. destruct (i <=? i); reflexivity.
+  intro. unfold max. simpl. rewrite Nat.max_id; reflexivity.
 Qed.
 Hint Rewrite interval_max_refl : soundness.
 
@@ -109,7 +108,7 @@ Proof.
   intros. unfold imult.
   assert (min i * min j <= max i * max j).
   apply Coq.Arith.Mult.mult_le_compat; apply interval_increasing.
-  unfold min at 1. simpl. apply Nat.leb_le in H. rewrite H. reflexivity.
+  unfold min, max in *. simpl. omega with *.
 Qed.
 
 Lemma interval_max_mult : forall i j,
@@ -117,5 +116,5 @@ Lemma interval_max_mult : forall i j,
 Proof. 
   intros. unfold imult. assert (min i * min j <= max i * max j).
   apply Coq.Arith.Mult.mult_le_compat; apply interval_increasing.
-  unfold max at 1. simpl. apply Nat.leb_le in H. rewrite H. reflexivity.
+  unfold min, max in *. simpl. omega with *.
 Qed.
