Types/Maybe.v
@@ -1,0 +1,49 @@
+Require Import Utf8.
+Require Import Classes.Monad.
+
+Inductive Maybe (A : Type) : Type :=
+    | Just : A -> Maybe A
+    | None : Maybe A.
+Arguments Just {_}.
+Arguments None {_}.
+
+Inductive AbstractMaybe (A : Type) : Type :=
+  | JustA : A -> AbstractMaybe A
+  | JustOrNoneA : A -> AbstractMaybe A
+  | NoneA : AbstractMaybe A.
+Arguments JustA {_}.
+Arguments JustOrNoneA {_}.
+Arguments NoneA {_}.
+
+Definition MaybeT (M : Type → Type) (A : Type) : Type := M (Maybe A).
+Section maybeT_laws.
+  Context {M} `{M_monad : Monad M}.
+  Definition NoneT {A} : MaybeT M A := returnM None.
+  Definition JustT {A} (a : A) : MaybeT M A := returnM (Just a).
+
+  Lemma justT_inj : ∀ A (x y : A),
+    JustT x = JustT y → x = y.
+  Proof.
+    intros A x y H. 
+    apply (returnM_inj (A:=Maybe A)) in H. inv H. reflexivity.
+  Qed.
+End maybeT_laws.
+
+Definition MaybeAT (M : Type → Type) (A : Type) : Type := M (AbstractMaybe A).
+
+Section maybeAT_laws.
+  Context {M} `{M_monad : Monad M}.
+
+  Definition NoneAT {A} : MaybeAT M A := returnM NoneA.
+  Definition JustAT {A} (a : A) : MaybeAT M A := 
+    returnM (JustA a).
+  Definition JustOrNoneAT {A} (a : A) : MaybeAT M A := 
+    returnM (JustOrNoneA a).
+
+  Lemma justAT_inj : ∀ A (x y : A),
+    JustAT x = JustAT y → x = y.
+  Proof.
+    intros A x y H. 
+    apply (returnM_inj (A:=AbstractMaybe A)) in H. inv H. reflexivity.
+  Qed.
+End maybeAT_laws.
