Types/State.v
@@ -1,0 +1,5 @@
+Require Import Utf8.
+
+Definition State (S A : Type) := S -> (A * S).
+Definition StateT S M A : Type := S → M (A*S)%type.
+
